\documentclass{article}

\usepackage{mathrsfs}
\usepackage{amsmath}
\usepackage{amssymb}
\usepackage[margin=0.5in]{geometry}

\newenvironment{myboxed}{\bigskip\noindent\begin{tabular}{|p{.975\textwidth}|}\hline \\}{\\\\\hline\end{tabular}\bigskip}
\newenvironment{mytitle}{\noindent\large\begin{flushright}}{\end{flushright}\normalsize}

\begin{document}

\begin{mytitle}
    Principles of Mathematical Analysis \\
    Chapter 6 \\
    \normalsize Jasper Ty
\end{mytitle}

\begin{myboxed}

\end{myboxed}

\begin{myboxed}
    \textsc{Riemann integral of $f \alpha'$ is equal to Riemann-Stieltjes integral of $f$ with integrator $\alpha$}
 
    \textbf{Theorem}

    Let $\alpha: [a,b] \rightarrow \mathbb{R}$ be a differentiable monotonic function such that $\alpha' \in \mathscr{R}$. Let $f: [a, b] \rightarrow \mathbb{R}$ be a bounded function. 

    Then $f \in \mathscr{R}(\alpha)$ if and only if $f\alpha' \in \mathscr{R}$. And
    \[\int_a^b fd\alpha = \int_a^b f(x) \alpha'(x) dx\]

    \textbf{Proof}

    Let $\varepsilon > 0$ and choose a partition $P$ such that
    \[U(P, \alpha') - L(P, \alpha') < \varepsilon\]
    If we pick any points $s_i, t_i \in [x_{i-1}, x_i]$, we have that
    \[\sum_{i=1}^n |\alpha'(s_i) - \alpha'(t_i)|\Delta x_i \leq \varepsilon \]
    Let $|f(x)| \leq M$, then
    \[\sum_{i=1}^n |\alpha'(s_i) \Delta x_i - \alpha'(t_i) \Delta x_i||f(s_i)| \leq  M\varepsilon \]
    Pushing the $f(s_i)$ in,
    \[\sum_{i=1}^n |f(s_i)\alpha'(s_i) \Delta x_i - f(s_i)\alpha'(t_i) \Delta x_i| \leq  M\varepsilon \]
    By the mean value theorem, we can choose $t_i$ such that
    \[\Delta\alpha_i = \alpha'(t_i)\Delta x_i\]
    Then
    \[\sum_{i=1}^n |f(s_i)\alpha'(s_i) \Delta x_i - f(s_i)\Delta\alpha_i| \leq  M\varepsilon \]
    By the triangle inequality,
    \[\left| \sum_{i=1}^n [f(s_i)\alpha'(s_i) \Delta x_i - f(s_i)\Delta\alpha_i] \right| \leq \sum_{i=1}^n |f(s_i)\alpha'(s_i) \Delta x_i - f(s_i)\Delta\alpha_i| \leq  M\varepsilon \]
    So 
    \[\left| \sum_{i=1}^n f(s_i)\alpha'(s_i) \Delta x_i - \sum_{i=1}^n f(s_i)\Delta\alpha_i \right| \leq \sum_{i=1}^n |f(s_i)\alpha'(s_i) \Delta x_i - f(s_i)\Delta\alpha_i| \leq  M\varepsilon \]
    In particular, letting $f(s_i)$ be $M_i$ and $m_i$ respectively,
    \[|U(P, f\alpha') - U(P, f, \alpha)| \leq M\varepsilon\]
    \[|L(P, f\alpha') - L(P, f, \alpha)| \leq M\varepsilon\]

\end{myboxed}

\begin{myboxed}
    Since the triangle inequality holds for $\sup$, consider the reverse triangle inequality (for $\sup$)
    \[\Bigg|\sup_P|U(P, f\alpha')| - \sup_P|U(P, f\alpha')|\Bigg|\leq \sup_P|U(P, f\alpha') - U(P, f, \alpha)| \leq M\varepsilon\]
    Then
    \[\left|\overline{\int_a^b}f\alpha'dx - \overline{\int_a^b}fd\alpha \right|\leq M\varepsilon\]
    Similarly,
    \[\left|\underline{\int_a^b}f\alpha'dx - \underline{\int_a^b}fd\alpha \right|\leq M\varepsilon\]
    Hence, if one integral exists, the other does. Moreover, their integrals are equal.
\end{myboxed}

\begin{myboxed}
    \textsc{Change of variable}

    \textbf{Theorem}
\end{myboxed}

\begin{myboxed}
    \textsc{Integration by parts}

    \textbf{Theorem}
\end{myboxed}

\end{document}
